Isotope/Syntax/Intrinsic.lean
@@ -1,2 +1,0 @@
-import Isotope.Syntax.Intrinsic.Basic
-import Isotope.Syntax.Intrinsic.Wk
