Isotope/Syntax/NamedList.lean
@@ -1,0 +1,2 @@
+import Isotope.Syntax.NamedList.Ctx
+import Isotope.Syntax.NamedList.LCtx
