Isotope/Syntax/NamedList/LCtx.lean
@@ -1,0 +1,56 @@
+import Isotope.Syntax.NamedList.Ctx
+
+namespace NamedList
+
+structure Label (T: Type u) where
+  name: String
+  live: Ctx T
+  param: Var T
+
+structure Label.wk {T: Type u} [HasLin T] (l k: Label T) where
+  name: l.name = k.name
+  live: l.live.wk k.live
+  param: l.param ≥ k.param
+
+def Label.wk.id {T: Type u} [HasLin T] (l: Label T): l.wk l where
+  name := rfl
+  live := Ctx.wk.id l.live
+  param := le_refl l.param
+
+def Label.wk.comp {T: Type u} [HasLin T] {l k j: Label T}
+  (Hlk: l.wk k) (Hkj: k.wk j): l.wk j where
+  name := Hlk.name.trans Hkj.name
+  live := Ctx.wk.comp Hlk.live Hkj.live
+  param := le_trans Hkj.param Hlk.param
+
+abbrev LCtx (T: Type u) := List (Label T)
+
+inductive LCtx.join {T: Type u} [HasLin T]: LCtx T -> LCtx T -> Type u
+  | nil: join [] []
+  | unreached {L K: LCtx T} (l: Label T): join L K -> join L (l :: K)
+  | cons {L K: LCtx T} {l l': Label T}
+    : l.wk l' -> join L K  -> join (l :: L) (l' :: K)
+
+-- inductive LCtx.sjoin {T: Type u} [HasLin T]: LCtx T -> LCtx T -> Type u
+--   | nil: sjoin [] []
+--   | cons {L K: LCtx T} (l: Label T): sjoin L K -> sjoin (l :: L) (l :: K)
+--   | unreached {L K: LCtx T} (l: Label T): sjoin L K -> sjoin L (l :: K)
+
+def LCtx.join.id {T: Type u} [HasLin T]: (L: LCtx T) -> LCtx.join L L
+  | [] => nil
+  | l :: L => cons (Label.wk.id l) (join.id L)
+
+def LCtx.join.comp {T: Type u} [HasLin T] {L K M: LCtx T}
+  : LCtx.join L K -> LCtx.join K M -> LCtx.join L M
+  | nil, j => j
+  | k, unreached l j => unreached l (comp k j)
+  | unreached _ j, cons H k => unreached _ (comp j k)
+  | cons H j, cons H' k => cons (Label.wk.comp H H') (comp j k)
+
+def LCtx.label {T: Type u} [HasLin T] (L: LCtx T) (l: Label T): Type u
+  := LCtx.join [l] L
+
+def LCtx.label.wk {T: Type u} [HasLin T] {L: LCtx T} {l k: Label T}
+  (W: l.wk k): L.label k -> L.label l
+  | join.unreached l' j => join.unreached l' (wk W j)
+  | join.cons W' j => join.cons (W.comp W') j
