Isotope/Syntax/Nameless.lean
@@ -1,0 +1,2 @@
+import Isotope.Syntax.Nameless.Basic
+import Isotope.Syntax.Nameless.Wk
