Isotope/Syntax/Untyped.lean
@@ -1,19 +1,30 @@
--- inductive SSA (I: Type)
--- -- Terms
--- | var (x: nat)
--- | op (f: F) (arg: SSA I)
--- | pair (l r: SSA I)
--- | let_tm (e a: SSA I)
--- | let2_tm (e a: SSA I)
--- | tt
--- | ff
--- | nil
--- -- Blocks
--- | br (l: Nat) (t: SSA I)
--- | ret (t: SSA I)
--- | let_blk (e a: SSA I)
--- | let2_blk (e a: SSA I)
--- | ite (e s t: SSA I)
--- | cfg (t: SSA I) (m: Nat) (L: Fin m -> SSA I)
--- -- Meta
--- | mvar (m: nat)
+inductive UntypedKind
+| term
+| block
+| cfg
+
+open UntypedKind
+
+inductive Untyped (I: Type u): UntypedKind -> Type u
+-- Terms
+| var (x: String): Untyped I term
+| op (f: F) (a: Untyped I term): Untyped I term
+| pair (l r: Untyped I term): Untyped I term
+| tt: Untyped I term
+| ff: Untyped I term
+| nil: Untyped I term
+-- Blocks
+| br (l: String) (t: Untyped I term): Untyped I block
+| ite (e: Untyped I term) (s t: Untyped I block): Untyped I block
+| cfg (t: Untyped I block) (C: Untyped I cfg): Untyped I block
+-- Let-bindings (shared)
+--TODO: add type annotations?
+| let1 (k: UntypedKind) (x: String) (e: Untyped I term) (t: Untyped I block)
+  : Untyped I k
+| let2 (k: UntypedKind) (x: String) (e: Untyped I term) (t: Untyped I block)
+  : Untyped I k
+-- Control-flow graphs
+| cfg_id: Untyped I cfg
+| cfg_def (C: Untyped I cfg) (l x: String) (t: Untyped I block): Untyped I cfg
+-- Meta
+| mvar (k: UntypedKind) (m: String): Untyped I k
